compiler/src/examples/FE310Compiler.v
@@ -149,24 +149,6 @@ Definition mcomp_sat:
   OStateND RiscvMachine unit -> RiscvMachine -> (RiscvMachine -> Prop) -> Prop :=
   GoFlatToRiscv.mcomp_sat.
 
-Lemma eq_empty: Lift1Prop.iff1 (eq (map.empty: mem)) (Separation.emp True).
-Proof.
-  split; intros.
-  - repeat split. congruence.
-  - destruct H. congruence.
-Qed.
-
-Lemma store_program_empty: forall prog addr,
-    program addr prog (unchecked_store_program addr prog map.empty).
-Proof.
-  intros.
-  pose proof (store_program RV32IM prog addr map.empty) as P.
-  SeparationLogic.seplog.
-  remember (program addr prog) as a. (* PARAMRECORDS *)
-  SeparationLogic.cancel_step.
-  apply eq_empty.
-Qed.
-
 Lemma undef_on_unchecked_store_byte_tuple_list:
   forall (n: nat) (l: list (HList.tuple word8 n)) (start: word32),
     map.undef_on (unchecked_store_byte_tuple_list start l map.empty)
